Parameterized heapsort

thys/examples/code/introsort.ll
@@ -1183,7 +1183,7 @@ define { i64, { i64, i8* } }* @Sorting_Introsort_str_sort_introsort_aux_impl({ i
     %tmpab = insertvalue { i64, { i64, i64 } } %xa, { i64, i64 } %tmpa, 1
     %xb = insertvalue { { i64, { i64, i8* } }*, { i64, { i64, i64 } } } zeroinitializer, { i64, { i64, i8* } }* %x, 0
     %x5 = insertvalue { { i64, { i64, i8* } }*, { i64, { i64, i64 } } } %xb, { i64, { i64, i64 } } %tmpab, 1
-    %x6 = call { i64, { i64, i8* } }* @Sorting_Introsort_str_sort_introsort_aux_impl_f_05535664 ({ { i64, { i64, i8* } }*, { i64, { i64, i64 } } } %x5)
+    %x6 = call { i64, { i64, i8* } }* @Sorting_Introsort_str_sort_introsort_aux_impl_f_011410114 ({ { i64, { i64, i8* } }*, { i64, { i64, i64 } } } %x5)
     ret { i64, { i64, i8* } }* %x6
 }
 
@@ -1351,7 +1351,7 @@ define i64* @introsort_aux(i64* %x, i64 %x1, i64 %x2, i64 %x3) {
     %tmpab = insertvalue { i64, { i64, i64 } } %xa, { i64, i64 } %tmpa, 1
     %xb = insertvalue { i64*, { i64, { i64, i64 } } } zeroinitializer, i64* %x, 0
     %x5 = insertvalue { i64*, { i64, { i64, i64 } } } %xb, { i64, { i64, i64 } } %tmpab, 1
-    %x6 = call i64* @Sorting_Introsort_unat_sort_introsort_aux_impl_f_05516446 ({ i64*, { i64, { i64, i64 } } } %x5)
+    %x6 = call i64* @Sorting_Introsort_unat_sort_introsort_aux_impl_f_011389204 ({ i64*, { i64, { i64, i64 } } } %x5)
     ret i64* %x6
 }
 
@@ -1701,7 +1701,36 @@ define i64* @Sorting_Introsort_unat_sort_guarded_insertion_sort_impl(i64 %x, i64
     ret i64* %a12
 }
 
-define { i64, { i64, i8* } }* @Sorting_Introsort_str_sort_introsort_aux_impl_f_05535664({ { i64, { i64, i8* } }*, { i64, { i64, i64 } } } %x) {
+define { i64, { i64, i8* } }* @Sorting_Introsort_str_sort_unguarded_insertion_sort_impl(i64 %x, i64 %x1, i64 %x2, { i64, { i64, i8* } }* %x3) {
+
+  start:
+    %x4 = insertvalue { { i64, { i64, i8* } }*, i64 } zeroinitializer, { i64, { i64, i8* } }* %x3, 0
+    %xa = insertvalue { { i64, { i64, i8* } }*, i64 } %x4, i64 %x1, 1
+    br label %while_start
+
+  while_start:
+    %xb = phi { { i64, { i64, i8* } }*, i64 } [ %x6, %while_body ], [ %xa, %start ]
+    %a1 = extractvalue { { i64, { i64, i8* } }*, i64 } %xb, 0
+    %a2 = extractvalue { { i64, { i64, i8* } }*, i64 } %xb, 1
+    %x5 = icmp slt i64 %a2, %x2
+    br i1 %x5, label %while_body, label %while_end
+
+  while_body:
+    %a11 = extractvalue { { i64, { i64, i8* } }*, i64 } %xb, 0
+    %a21 = extractvalue { { i64, { i64, i8* } }*, i64 } %xb, 1
+    %xaa = call { i64, { i64, i8* } }* @Sorting_Introsort_str_sort_is_unguarded_insert_impl ({ i64, { i64, i8* } }* %a11, i64 %x, i64 %a21)
+    %xba = add i64 %a21, 1
+    %xca = insertvalue { { i64, { i64, i8* } }*, i64 } zeroinitializer, { i64, { i64, i8* } }* %xaa, 0
+    %x6 = insertvalue { { i64, { i64, i8* } }*, i64 } %xca, i64 %xba, 1
+    br label %while_start
+
+  while_end:
+    %a12 = extractvalue { { i64, { i64, i8* } }*, i64 } %xb, 0
+    %a22 = extractvalue { { i64, { i64, i8* } }*, i64 } %xb, 1
+    ret { i64, { i64, i8* } }* %a12
+}
+
+define { i64, { i64, i8* } }* @Sorting_Introsort_str_sort_introsort_aux_impl_f_011410114({ { i64, { i64, i8* } }*, { i64, { i64, i64 } } } %x) {
 
   start:
     %a1 = extractvalue { { i64, { i64, i8* } }*, { i64, { i64, i64 } } } %x, 0
@@ -1884,7 +1913,7 @@ define { i64, { i64, i8* } }* @Sorting_Introsort_str_sort_introsort_aux_impl_f_0
     %tmpga = insertvalue { i64, { i64, i64 } } %yb, { i64, i64 } %tmpfa, 1
     %yc = insertvalue { { i64, { i64, i8* } }*, { i64, { i64, i64 } } } zeroinitializer, { i64, { i64, i8* } }* %a1ca, 0
     %yd = insertvalue { { i64, { i64, i8* } }*, { i64, { i64, i64 } } } %yc, { i64, { i64, i64 } } %tmpga, 1
-    %yaa = call { i64, { i64, i8* } }* @Sorting_Introsort_str_sort_introsort_aux_impl_f_05535664 ({ { i64, { i64, i8* } }*, { i64, { i64, i64 } } } %yd)
+    %yaa = call { i64, { i64, i8* } }* @Sorting_Introsort_str_sort_introsort_aux_impl_f_011410114 ({ { i64, { i64, i8* } }*, { i64, { i64, i64 } } } %yd)
     %yba = sub i64 %a2b, 1
     %yf2 = insertvalue { i64, i64 } zeroinitializer, i64 %a1b, 0
     %tmphb = insertvalue { i64, i64 } %yf2, i64 %yba, 1
@@ -1892,7 +1921,7 @@ define { i64, { i64, i8* } }* @Sorting_Introsort_str_sort_introsort_aux_impl_f_0
     %tmpia = insertvalue { i64, { i64, i64 } } %yg2, { i64, i64 } %tmphb, 1
     %yh2 = insertvalue { { i64, { i64, i8* } }*, { i64, { i64, i64 } } } zeroinitializer, { i64, { i64, i8* } }* %yaa, 0
     %x12 = insertvalue { { i64, { i64, i8* } }*, { i64, { i64, i64 } } } %yh2, { i64, { i64, i64 } } %tmpia, 1
-    %x13 = call { i64, { i64, i8* } }* @Sorting_Introsort_str_sort_introsort_aux_impl_f_05535664 ({ { i64, { i64, i8* } }*, { i64, { i64, i64 } } } %x12)
+    %x13 = call { i64, { i64, i8* } }* @Sorting_Introsort_str_sort_introsort_aux_impl_f_011410114 ({ { i64, { i64, i8* } }*, { i64, { i64, i64 } } } %x12)
     br label %ctd_ifa
 
   ctd_ifa:
@@ -1907,36 +1936,36 @@ define { i64, { i64, i8* } }* @Sorting_Introsort_str_sort_introsort_aux_impl_f_0
     ret { i64, { i64, i8* } }* %x15
 }
 
-define { i64, { i64, i8* } }* @Sorting_Introsort_str_sort_unguarded_insertion_sort_impl(i64 %x, i64 %x1, i64 %x2, { i64, { i64, i8* } }* %x3) {
+define i64* @Sorting_Introsort_unat_sort_unguarded_insertion_sort_impl(i64 %x, i64 %x1, i64 %x2, i64* %x3) {
 
   start:
-    %x4 = insertvalue { { i64, { i64, i8* } }*, i64 } zeroinitializer, { i64, { i64, i8* } }* %x3, 0
-    %xa = insertvalue { { i64, { i64, i8* } }*, i64 } %x4, i64 %x1, 1
+    %x4 = insertvalue { i64*, i64 } zeroinitializer, i64* %x3, 0
+    %xa = insertvalue { i64*, i64 } %x4, i64 %x1, 1
     br label %while_start
 
   while_start:
-    %xb = phi { { i64, { i64, i8* } }*, i64 } [ %x6, %while_body ], [ %xa, %start ]
-    %a1 = extractvalue { { i64, { i64, i8* } }*, i64 } %xb, 0
-    %a2 = extractvalue { { i64, { i64, i8* } }*, i64 } %xb, 1
+    %xb = phi { i64*, i64 } [ %x6, %while_body ], [ %xa, %start ]
+    %a1 = extractvalue { i64*, i64 } %xb, 0
+    %a2 = extractvalue { i64*, i64 } %xb, 1
     %x5 = icmp slt i64 %a2, %x2
     br i1 %x5, label %while_body, label %while_end
 
   while_body:
-    %a11 = extractvalue { { i64, { i64, i8* } }*, i64 } %xb, 0
-    %a21 = extractvalue { { i64, { i64, i8* } }*, i64 } %xb, 1
-    %xaa = call { i64, { i64, i8* } }* @Sorting_Introsort_str_sort_is_unguarded_insert_impl ({ i64, { i64, i8* } }* %a11, i64 %x, i64 %a21)
+    %a11 = extractvalue { i64*, i64 } %xb, 0
+    %a21 = extractvalue { i64*, i64 } %xb, 1
+    %xaa = call i64* @Sorting_Introsort_unat_sort_is_unguarded_insert_impl (i64* %a11, i64 %x, i64 %a21)
     %xba = add i64 %a21, 1
-    %xca = insertvalue { { i64, { i64, i8* } }*, i64 } zeroinitializer, { i64, { i64, i8* } }* %xaa, 0
-    %x6 = insertvalue { { i64, { i64, i8* } }*, i64 } %xca, i64 %xba, 1
+    %xca = insertvalue { i64*, i64 } zeroinitializer, i64* %xaa, 0
+    %x6 = insertvalue { i64*, i64 } %xca, i64 %xba, 1
     br label %while_start
 
   while_end:
-    %a12 = extractvalue { { i64, { i64, i8* } }*, i64 } %xb, 0
-    %a22 = extractvalue { { i64, { i64, i8* } }*, i64 } %xb, 1
-    ret { i64, { i64, i8* } }* %a12
+    %a12 = extractvalue { i64*, i64 } %xb, 0
+    %a22 = extractvalue { i64*, i64 } %xb, 1
+    ret i64* %a12
 }
 
-define i64* @Sorting_Introsort_unat_sort_introsort_aux_impl_f_05516446({ i64*, { i64, { i64, i64 } } } %x) {
+define i64* @Sorting_Introsort_unat_sort_introsort_aux_impl_f_011389204({ i64*, { i64, { i64, i64 } } } %x) {
 
   start:
     %a1 = extractvalue { i64*, { i64, { i64, i64 } } } %x, 0
@@ -2119,7 +2148,7 @@ define i64* @Sorting_Introsort_unat_sort_introsort_aux_impl_f_05516446({ i64*, {
     %tmpga = insertvalue { i64, { i64, i64 } } %yb, { i64, i64 } %tmpfa, 1
     %yc = insertvalue { i64*, { i64, { i64, i64 } } } zeroinitializer, i64* %a1ca, 0
     %yd = insertvalue { i64*, { i64, { i64, i64 } } } %yc, { i64, { i64, i64 } } %tmpga, 1
-    %yaa = call i64* @Sorting_Introsort_unat_sort_introsort_aux_impl_f_05516446 ({ i64*, { i64, { i64, i64 } } } %yd)
+    %yaa = call i64* @Sorting_Introsort_unat_sort_introsort_aux_impl_f_011389204 ({ i64*, { i64, { i64, i64 } } } %yd)
     %yba = sub i64 %a2b, 1
     %yf2 = insertvalue { i64, i64 } zeroinitializer, i64 %a1b, 0
     %tmphb = insertvalue { i64, i64 } %yf2, i64 %yba, 1
@@ -2127,7 +2156,7 @@ define i64* @Sorting_Introsort_unat_sort_introsort_aux_impl_f_05516446({ i64*, {
     %tmpia = insertvalue { i64, { i64, i64 } } %yg2, { i64, i64 } %tmphb, 1
     %yh2 = insertvalue { i64*, { i64, { i64, i64 } } } zeroinitializer, i64* %yaa, 0
     %x12 = insertvalue { i64*, { i64, { i64, i64 } } } %yh2, { i64, { i64, i64 } } %tmpia, 1
-    %x13 = call i64* @Sorting_Introsort_unat_sort_introsort_aux_impl_f_05516446 ({ i64*, { i64, { i64, i64 } } } %x12)
+    %x13 = call i64* @Sorting_Introsort_unat_sort_introsort_aux_impl_f_011389204 ({ i64*, { i64, { i64, i64 } } } %x12)
     br label %ctd_ifa
 
   ctd_ifa:
@@ -2140,33 +2169,4 @@ define i64* @Sorting_Introsort_unat_sort_introsort_aux_impl_f_05516446({ i64*, {
   ctd_if:
     %x15 = phi i64* [ %a1, %else ], [ %x14, %ctd_ifa ]
     ret i64* %x15
-}
-
-define i64* @Sorting_Introsort_unat_sort_unguarded_insertion_sort_impl(i64 %x, i64 %x1, i64 %x2, i64* %x3) {
-
-  start:
-    %x4 = insertvalue { i64*, i64 } zeroinitializer, i64* %x3, 0
-    %xa = insertvalue { i64*, i64 } %x4, i64 %x1, 1
-    br label %while_start
-
-  while_start:
-    %xb = phi { i64*, i64 } [ %x6, %while_body ], [ %xa, %start ]
-    %a1 = extractvalue { i64*, i64 } %xb, 0
-    %a2 = extractvalue { i64*, i64 } %xb, 1
-    %x5 = icmp slt i64 %a2, %x2
-    br i1 %x5, label %while_body, label %while_end
-
-  while_body:
-    %a11 = extractvalue { i64*, i64 } %xb, 0
-    %a21 = extractvalue { i64*, i64 } %xb, 1
-    %xaa = call i64* @Sorting_Introsort_unat_sort_is_unguarded_insert_impl (i64* %a11, i64 %x, i64 %a21)
-    %xba = add i64 %a21, 1
-    %xca = insertvalue { i64*, i64 } zeroinitializer, i64* %xaa, 0
-    %x6 = insertvalue { i64*, i64 } %xca, i64 %xba, 1
-    br label %while_start
-
-  while_end:
-    %a12 = extractvalue { i64*, i64 } %xb, 0
-    %a22 = extractvalue { i64*, i64 } %xb, 1
-    ret i64* %a12
 }
