thys/examples/sorting/Sorting_Setup.thy
@@ -321,9 +321,6 @@ begin
     apply auto
     done
 
-  (* TODO: Move *)
-  lemma unborrow_nofail[refine_pw_simps]: "nofail (unborrow a b) \<longleftrightarrow> a=b" by (auto simp: unborrow_def refine_pw_simps)  
-    
   lemma cmp_idxs2_refine: "(uncurry2 cmp_idxs2,uncurry2 (PR_CONST mop_cmp_idxs))\<in>[\<lambda>((xs,i),j). i\<noteq>j]\<^sub>f (Id\<times>\<^sub>rId)\<times>\<^sub>rId \<rightarrow> \<langle>Id\<rangle>nres_rel"
     unfolding cmp_idxs2_def mop_cmp_idxs_def PR_CONST_def
     apply (intro frefI nres_relI)
@@ -469,19 +466,424 @@ lemma unat_sort_impl_context: "pure_sort_impl_context (\<le>) (<) ll_icmp_ult un
   done
   
   
+subsection \<open>Parameterized Sorting\<close>  
+
+text \<open>Extension of a weak ordering with explicit carrier set is always possible, 
+  e.g., by putting all elements not in the carrier set into one equivalence class,
+  which is smaller than any other class.\<close>  
+locale weak_ordering_on_lt =
+  fixes C :: "'a set"
+    and less :: "'a \<Rightarrow> 'a \<Rightarrow> bool" (infix "\<^bold><" 50)
+  assumes asym: "\<lbrakk> a\<in>C; b\<in>C \<rbrakk> \<Longrightarrow> a\<^bold><b \<Longrightarrow> \<not>b\<^bold><a"
+  assumes itrans: "\<lbrakk> a\<in>C; b\<in>C; c\<in>C \<rbrakk> \<Longrightarrow> a\<^bold><c \<Longrightarrow> a\<^bold><b \<or> b\<^bold><c"
+
+definition "ext_lt C lt a b \<equiv> lt a b \<and> a\<in>C \<and> b\<in>C \<or> a\<in>C \<and> b\<notin>C"  
+  
+lemma weak_ordering_on_lt_extend: "weak_ordering_lt (ext_lt C lt) \<longleftrightarrow> weak_ordering_on_lt C lt"
+  unfolding weak_ordering_on_lt_def weak_ordering_lt_def ext_lt_def
+  by blast
   
   
+(* TODO: Restrict cdom constraint to slice! *)
+definition "pslice_sort_spec cdom pless cparam xs l h \<equiv> doN {
+  \<^cancel>\<open>ASSERT (set (slice l h xs) \<subseteq> cdom cparam);\<close>
+  ASSERT (set xs \<subseteq> cdom cparam);
+  slice_sort_spec (pless cparam) xs l h
+}"  
+  
+
+locale parameterized_weak_ordering1 =
+  fixes cdom :: "'cparam \<Rightarrow> 'a set"
+    and pless :: "'cparam \<Rightarrow> 'a \<Rightarrow> 'a \<Rightarrow> bool"
+    and pcmp :: "'cparam \<Rightarrow> 'a \<Rightarrow> 'a \<Rightarrow> bool nres"
+  assumes weak_ordering_on_lt: "weak_ordering_on_lt (cdom cparam) (pless cparam)"
+  assumes pcmp_correct[refine_vcg]: "\<lbrakk> a\<in>cdom cparam; b\<in>cdom cparam\<rbrakk> 
+    \<Longrightarrow> pcmp cparam a b \<le> SPEC (\<lambda>r. r \<longleftrightarrow> pless cparam a b)"
+begin    
+
+  definition "cdom_rel cparam \<equiv> br id (\<lambda>x. x\<in>cdom cparam)"
+  definition "cdom_list_rel cparam \<equiv> \<langle>cdom_rel cparam\<rangle>list_rel"
+  definition "cdom_olist_rel cparam \<equiv> \<langle>\<langle>cdom_rel cparam\<rangle>option_rel\<rangle>list_rel"
+  
+  lemma br_id_list_rel_conv: "(xs,xs')\<in>\<langle>br id I\<rangle>list_rel \<longleftrightarrow> xs=xs' \<and> set xs' \<subseteq> Collect I"
+    apply (induction xs arbitrary: xs')
+    subgoal for xs' by (auto)
+    subgoal for x xs xs' by (cases xs') (auto simp: in_br_conv)
+    done  
+  
+  lemma br_id_olist_rel_conv: "(xs,xs')\<in>\<langle>\<langle>br id I\<rangle>option_rel\<rangle>list_rel \<longleftrightarrow> xs=xs' \<and> (\<forall>x. Some x\<in>set xs' \<longrightarrow> I x)"
+    apply (induction xs arbitrary: xs')
+    subgoal for xs' by (auto)
+    subgoal for x xs xs' by (cases xs') (auto simp: in_br_conv option_rel_def)
+    done  
+  
+  lemma cdom_list_rel_alt: "cdom_list_rel cparam = br id (\<lambda>xs. set xs \<subseteq> cdom cparam)"
+    unfolding cdom_list_rel_def cdom_rel_def
+    by (auto simp: in_br_conv br_id_list_rel_conv)
+  
+  lemma cdom_olist_rel_alt: "cdom_olist_rel cparam = br id (\<lambda>xs. \<forall>x. Some x \<in> set xs \<longrightarrow> x\<in>cdom cparam)"
+    unfolding cdom_olist_rel_def cdom_rel_def
+    by (auto simp: in_br_conv br_id_olist_rel_conv)
+
+  definition "less' cparam \<equiv> (ext_lt (cdom cparam) (pless cparam))"
+
+  lemma weak_ordering_lt: "weak_ordering_lt (less' cparam)" 
+    using weak_ordering_on_lt less'_def by (simp add: weak_ordering_on_lt_extend) 
+
+  lemma weak_ordering: "weak_ordering (le_by_lt (less' cparam)) (less' cparam)"
+  proof -
+    interpret weak_ordering_lt "less' cparam" by (rule weak_ordering_lt)
+    show ?thesis by unfold_locales
+  qed      
+
+  sublocale WO: weak_ordering "le_by_lt (less' cparam)" "less' cparam"
+    by (rule weak_ordering)
   
   
+  lemma sorted_wrt_ext: "set xs \<subseteq> cdom cparam \<Longrightarrow> sorted_wrt (less' cparam) xs = sorted_wrt (pless cparam) xs"
+    apply (intro iffI; erule sorted_wrt_mono_rel[rotated])
+    apply (auto simp: less'_def ext_lt_def)
+    done
   
+  (* TODO: Move *)  
+  lemma set_slice_ss: "set (slice l h xs) \<subseteq> set xs"  
+    by (metis Misc.slice_def dual_order.trans set_drop_subset set_take_subset)
+    
+  lemma slice_sort_spec_xfer: "\<Down> (cdom_list_rel cparam) (slice_sort_spec (less' cparam) xs l h) \<le> pslice_sort_spec cdom pless cparam xs l h"
+    unfolding pslice_sort_spec_def cdom_list_rel_alt 
+    apply (auto simp: pw_le_iff refine_pw_simps in_br_conv)
+    unfolding slice_sort_spec_alt
+    apply (auto simp: refine_pw_simps)
+    using sorted_wrt_ext
+    by (smt ext_lt_def le_by_lt_def less'_def set_slice_ss sorted_wrt_mono_rel subsetD)
+    
 (*
-(* TODO: Refine lemmas to support more general datatypes! *)
-type_synonym elem_t = "64"
+  lemma pslice_sort_spec_xfer:
+    assumes "m \<le> slice_sort_spec (less' cparam) xs l h"
+    assumes "mm \<le> \<Down>(cdom_list_rel cparam) m"
+    assumes "(xs',xs)\<in>cdom_list_rel cparam"
+    shows "mm \<le> pslice_sort_spec cdom pless cparam xs l h"
+    using assms unfolding pslice_sort_spec_def cdom_list_rel_alt 
+    apply (auto simp: pw_le_iff refine_pw_simps in_br_conv)
+    unfolding slice_sort_spec_alt
+    apply (auto simp: refine_pw_simps)
+    using sorted_wrt_ext
+    by (smt ext_lt_def le_by_lt_def less'_def set_slice_ss sorted_wrt_mono_rel subset_code(1))
+*)  
 
-abbreviation "elem_assn \<equiv> unat_assn' TYPE(elem_t)"
+    
+    
+    
+  lemma olist_to_eo_conv_refine[refine]: 
+    "(xs',xs)\<in>cdom_list_rel cparam \<Longrightarrow> mop_to_eo_conv xs' \<le> \<Down>(cdom_olist_rel cparam) (mop_to_eo_conv xs)"
+    apply (rule nres_relD)
+    unfolding mop_to_eo_conv_def cdom_olist_rel_def cdom_list_rel_def
+    by (parametricity)
+    
+  lemma olist_to_wo_conv_refine[refine]: 
+    "\<lbrakk>(xs',xs)\<in>cdom_olist_rel cparam\<rbrakk> \<Longrightarrow> mop_to_wo_conv xs' \<le> \<Down>(cdom_list_rel cparam) (mop_to_wo_conv xs)"
+    apply simp
+    apply refine_rcg
+    apply (auto simp: cdom_olist_rel_alt cdom_list_rel_alt in_br_conv)
+    by (metis option.collapse)
 
-abbreviation "arr_assn \<equiv> array_assn elem_assn"
+    
+  lemma olist_extract_refine[refine]: "\<lbrakk> (xs',xs)\<in>cdom_olist_rel cparam; (i',i)\<in>Id \<rbrakk> 
+    \<Longrightarrow> mop_eo_extract xs' i' \<le> \<Down> ((br id (\<lambda>x. x\<in>cdom cparam)) \<times>\<^sub>r cdom_olist_rel cparam) (mop_eo_extract xs i)"
+    unfolding mop_eo_extract_alt
+    apply refine_vcg
+    apply (auto simp: cdom_olist_rel_alt in_br_conv)
+    by (metis in_set_upd_cases option.distinct(1))
+    
+  lemma listo_eo_set_refine[refine]: "\<lbrakk>
+    (xs',xs)\<in>cdom_olist_rel cparam;
+    (i',i)\<in>Id;
+    (v',v)\<in>Id; v\<in>cdom cparam
+  \<rbrakk> \<Longrightarrow> mop_eo_set xs' i' v' \<le> \<Down> (cdom_olist_rel cparam) (mop_eo_set xs i v)"  
+    apply simp
+    apply refine_vcg
+    apply (auto simp: cdom_olist_rel_alt in_br_conv)
+    by (metis in_set_upd_cases option.sel)
+
+    
+  definition "pcmpo_idxs2 cparam xs\<^sub>0 i j \<equiv> doN {
+    ASSERT (i \<noteq> j);
+    (vi,xs) \<leftarrow> mop_eo_extract xs\<^sub>0 i;
+    (vj,xs) \<leftarrow> mop_eo_extract xs j;
+    r \<leftarrow> pcmp cparam vi vj;
+    xs \<leftarrow> mop_eo_set xs i vi; \<comment> \<open>TODO: Let's hope the optimizer eliminates these assignments. In mid-term, eliminate them during sepref phase!\<close>
+    xs \<leftarrow> mop_eo_set xs j vj;
+    unborrow xs xs\<^sub>0;
+    RETURN r
+  }"
+    
+  definition "pcmpo_v_idx2 cparam xs\<^sub>0 v j \<equiv> doN {
+    (vj,xs) \<leftarrow> mop_eo_extract xs\<^sub>0 j;
+    r \<leftarrow> pcmp cparam v vj;
+    xs \<leftarrow> mop_eo_set xs j vj;
+    unborrow xs xs\<^sub>0;
+    RETURN r
+  }"
+
+  definition "pcmpo_idx_v2 cparam xs\<^sub>0 i v \<equiv> doN {
+    (vi,xs) \<leftarrow> mop_eo_extract xs\<^sub>0 i;
+    r \<leftarrow> pcmp cparam vi v;
+    xs \<leftarrow> mop_eo_set xs i vi;
+    unborrow xs xs\<^sub>0;
+    RETURN r
+  }"
+
+  definition "pcmp_idxs2 cparam xs\<^sub>0 i j \<equiv> doN {
+    xs \<leftarrow> mop_to_eo_conv xs\<^sub>0;
+    b \<leftarrow> pcmpo_idxs2 cparam xs i j;
+    xs \<leftarrow> mop_to_wo_conv xs;
+    unborrow xs xs\<^sub>0;
+    RETURN b
+  }"  
+  
+  lemma pcmpo_idxs_refine[refine]: "\<lbrakk>
+    (xs',xs)\<in> cdom_olist_rel cparam;
+    i\<noteq>j;
+    (i',i)\<in>Id;
+    (j',j)\<in>Id
+  \<rbrakk> \<Longrightarrow> pcmpo_idxs2 cparam xs' i' j' \<le> \<Down> bool_rel (WO.mop_cmpo_idxs cparam xs i j)"  
+    unfolding pcmpo_idxs2_def
+    apply simp
+    apply refine_vcg
+    apply (auto simp: cdom_olist_rel_alt in_br_conv less'_def ext_lt_def
+           list_update_swap[of i j] map_update[symmetric])
+    done
+  
+  
+  lemma pcmpo_v_idx_refine[refine]: "\<lbrakk>
+    (xs',xs)\<in> cdom_olist_rel cparam;
+    (v',v)\<in>Id; v\<in>cdom cparam;
+    (i',i)\<in>Id
+  \<rbrakk> \<Longrightarrow> pcmpo_v_idx2 cparam xs' v' i' \<le> \<Down> bool_rel (WO.mop_cmpo_v_idx cparam xs v i)"  
+    unfolding pcmpo_v_idx2_def
+    apply simp
+    apply refine_vcg
+    apply (auto simp: cdom_olist_rel_alt in_br_conv less'_def ext_lt_def)
+    done
+    
+  lemma pcmpo_idx_v_refine[refine]: "\<lbrakk>
+    (xs',xs)\<in> cdom_olist_rel cparam;
+    (v',v)\<in>Id; v\<in>cdom cparam;
+    (i',i)\<in>Id
+  \<rbrakk> \<Longrightarrow> pcmpo_idx_v2 cparam xs' i' v' \<le> \<Down> bool_rel (WO.mop_cmpo_idx_v cparam xs i v)"  
+    unfolding pcmpo_idx_v2_def
+    apply simp
+    apply refine_vcg
+    apply (auto simp: cdom_olist_rel_alt in_br_conv less'_def ext_lt_def)
+    done
+  
+  lemma pcmp_idxs_refine[refine]: "\<lbrakk>
+    (xs',xs)\<in> cdom_list_rel cparam;
+    i\<noteq>j;
+    (i',i)\<in>Id;
+    (j',j)\<in>Id
+  \<rbrakk> \<Longrightarrow> pcmp_idxs2 cparam xs' i' j' \<le> \<Down> bool_rel (WO.mop_cmp_idxs cparam xs i j)"  
+    unfolding pcmp_idxs2_def pcmpo_idxs2_def
+    apply simp
+    apply refine_vcg
+    apply (auto 0 3 simp: cdom_list_rel_alt in_br_conv less'_def ext_lt_def 
+           list_update_swap[of i j] map_update[symmetric])
+    using nth_mem by blast
+    
+    
+    
+end
+
+(*
+locale parameterized_weak_ordering = weak_ordering +
+  fixes (*cparam :: 'cparam*)
+        cdom :: "'cparam \<Rightarrow> 'a set"
+    and pcmp :: "'cparam \<Rightarrow> 'a \<Rightarrow> 'a \<Rightarrow> bool nres"
+  assumes pcmp_correct[refine_vcg]: "\<lbrakk> a\<in>cdom cparam; b\<in>cdom cparam\<rbrakk> 
+    \<Longrightarrow> pcmp cparam a b \<le> SPEC (\<lambda>r. r \<longleftrightarrow> a\<^bold><b)"
+    
+    
+    
+begin
+  (* TODO: The refinements established here are just a special case of list-element refinement.
+    We should use list-rel here! And generic parametricity lemmas from the operations!
+  *)
+  definition "cdom_list_rel cparam \<equiv> br id (\<lambda>xs. set xs \<subseteq> cdom cparam)"
+  definition "cdom_olist_rel cparam \<equiv> br id (\<lambda>xs. \<forall>x. Some x \<in> set xs \<longrightarrow> x\<in>cdom cparam)"
+
+  lemma olist_to_eo_conv_refine[refine]: 
+    "(xs',xs)\<in>cdom_list_rel cparam \<Longrightarrow> mop_to_eo_conv xs' \<le> \<Down>(cdom_olist_rel cparam) (mop_to_eo_conv xs)"
+    unfolding mop_to_eo_conv_def cdom_list_rel_def cdom_olist_rel_def
+    by (auto simp: in_br_conv)
+    
+  lemma olist_to_wo_conv_refine[refine]: 
+    "\<lbrakk>(xs',xs)\<in>cdom_olist_rel cparam\<rbrakk> \<Longrightarrow> mop_to_wo_conv xs' \<le> \<Down>(cdom_list_rel cparam) (mop_to_wo_conv xs)"
+    apply simp
+    apply refine_rcg
+    apply (auto simp: cdom_olist_rel_def cdom_list_rel_def in_br_conv)
+    by (metis option.collapse)
+
+    
+  lemma olist_extract_refine[refine]: "\<lbrakk> (xs',xs)\<in>cdom_olist_rel cparam; (i',i)\<in>Id \<rbrakk> 
+    \<Longrightarrow> mop_eo_extract xs' i' \<le> \<Down> ((br id (\<lambda>x. x\<in>cdom cparam)) \<times>\<^sub>r cdom_olist_rel cparam) (mop_eo_extract xs i)"
+    unfolding mop_eo_extract_alt
+    apply refine_vcg
+    apply (auto simp: cdom_olist_rel_def in_br_conv)
+    by (metis in_set_upd_cases option.distinct(1))
+    
+  lemma listo_eo_set_refine[refine]: "\<lbrakk>
+    (xs',xs)\<in>cdom_olist_rel cparam;
+    (i',i)\<in>Id;
+    (v',v)\<in>Id; v\<in>cdom cparam
+  \<rbrakk> \<Longrightarrow> mop_eo_set xs' i' v' \<le> \<Down> (cdom_olist_rel cparam) (mop_eo_set xs i v)"  
+    apply simp
+    apply refine_vcg
+    apply (auto simp: cdom_olist_rel_def in_br_conv)
+    by (metis in_set_upd_cases option.sel)
+
+    
+  definition "pcmpo_idxs2 cparam xs\<^sub>0 i j \<equiv> doN {
+    ASSERT (i \<noteq> j);
+    (vi,xs) \<leftarrow> mop_eo_extract xs\<^sub>0 i;
+    (vj,xs) \<leftarrow> mop_eo_extract xs j;
+    r \<leftarrow> pcmp cparam vi vj;
+    xs \<leftarrow> mop_eo_set xs i vi; \<comment> \<open>TODO: Let's hope the optimizer eliminates these assignments. In mid-term, eliminate them during sepref phase!\<close>
+    xs \<leftarrow> mop_eo_set xs j vj;
+    unborrow xs xs\<^sub>0;
+    RETURN r
+  }"
+    
+  definition "pcmpo_v_idx2 cparam xs\<^sub>0 v j \<equiv> doN {
+    (vj,xs) \<leftarrow> mop_eo_extract xs\<^sub>0 j;
+    r \<leftarrow> pcmp cparam v vj;
+    xs \<leftarrow> mop_eo_set xs j vj;
+    unborrow xs xs\<^sub>0;
+    RETURN r
+  }"
+
+  definition "pcmpo_idx_v2 cparam xs\<^sub>0 i v \<equiv> doN {
+    (vi,xs) \<leftarrow> mop_eo_extract xs\<^sub>0 i;
+    r \<leftarrow> pcmp cparam vi v;
+    xs \<leftarrow> mop_eo_set xs i vi;
+    unborrow xs xs\<^sub>0;
+    RETURN r
+  }"
+
+  definition "pcmp_idxs2 cparam xs\<^sub>0 i j \<equiv> doN {
+    xs \<leftarrow> mop_to_eo_conv xs\<^sub>0;
+    b \<leftarrow> pcmpo_idxs2 cparam xs i j;
+    xs \<leftarrow> mop_to_wo_conv xs;
+    unborrow xs xs\<^sub>0;
+    RETURN b
+  }"  
+  
+  lemma pcmpo_idxs_refine[refine]: "\<lbrakk>
+    (xs',xs)\<in> cdom_olist_rel cparam;
+    i\<noteq>j;
+    (i',i)\<in>Id;
+    (j',j)\<in>Id
+  \<rbrakk> \<Longrightarrow> pcmpo_idxs2 cparam xs' i' j' \<le> \<Down> bool_rel (mop_cmpo_idxs xs i j)"  
+    unfolding pcmpo_idxs2_def
+    apply simp
+    apply refine_vcg
+    apply (auto simp: cdom_olist_rel_def in_br_conv 
+           list_update_swap[of i j] map_update[symmetric])
+    done
+  
+  
+  lemma pcmpo_v_idx_refine[refine]: "\<lbrakk>
+    (xs',xs)\<in> cdom_olist_rel cparam;
+    (v',v)\<in>Id; v\<in>cdom cparam;
+    (i',i)\<in>Id
+  \<rbrakk> \<Longrightarrow> pcmpo_v_idx2 cparam xs' v' i' \<le> \<Down> bool_rel (mop_cmpo_v_idx xs v i)"  
+    unfolding pcmpo_v_idx2_def
+    apply simp
+    apply refine_vcg
+    apply (auto simp: cdom_olist_rel_def in_br_conv)
+    done
+    
+  lemma pcmpo_idx_v_refine[refine]: "\<lbrakk>
+    (xs',xs)\<in> cdom_olist_rel cparam;
+    (v',v)\<in>Id; v\<in>cdom cparam;
+    (i',i)\<in>Id
+  \<rbrakk> \<Longrightarrow> pcmpo_idx_v2 cparam xs' i' v' \<le> \<Down> bool_rel (mop_cmpo_idx_v xs i v)"  
+    unfolding pcmpo_idx_v2_def
+    apply simp
+    apply refine_vcg
+    apply (auto simp: cdom_olist_rel_def in_br_conv)
+    done
+  
+  lemma pcmp_idxs_refine[refine]: "\<lbrakk>
+    (xs',xs)\<in> cdom_list_rel cparam;
+    i\<noteq>j;
+    (i',i)\<in>Id;
+    (j',j)\<in>Id
+  \<rbrakk> \<Longrightarrow> pcmp_idxs2 cparam xs' i' j' \<le> \<Down> bool_rel (mop_cmp_idxs xs i j)"  
+    unfolding pcmp_idxs2_def pcmpo_idxs2_def
+    apply simp
+    apply refine_vcg
+    apply (auto 0 3 simp: cdom_list_rel_def in_br_conv
+           list_update_swap[of i j] map_update[symmetric])
+    done
+    
+    
+end
 *)
+
+text \<open>The compare function takes an external parameter.\<close>  
+
+
+definition "refines_param_relp P A R Rimpl \<equiv> (uncurry2 Rimpl,uncurry2 R) \<in> P\<^sup>k*\<^sub>aA\<^sup>k*\<^sub>aA\<^sup>k\<rightarrow>\<^sub>abool1_assn"
+
+lemma gen_refines_param_relpD: "GEN_ALGO Rimpl (refines_param_relp P A R) 
+  \<Longrightarrow> (uncurry2 Rimpl,uncurry2 R) \<in> P\<^sup>k*\<^sub>aA\<^sup>k*\<^sub>aA\<^sup>k\<rightarrow>\<^sub>abool1_assn"
+  by (simp add: GEN_ALGO_def refines_param_relp_def)
+
+
+locale parameterized_sort_impl_context = parameterized_weak_ordering1 +
+  constrains "cdom" :: "'cparam \<Rightarrow> _" and pless :: _ and pcmp :: "'cparam \<Rightarrow> 'a \<Rightarrow> 'a \<Rightarrow> bool nres"
+  fixes pcmp_impl :: "'cparami \<Rightarrow> 'ai::llvm_rep \<Rightarrow> 'ai \<Rightarrow> 1 word llM"
+    and cparam_assn :: "'cparam \<Rightarrow> 'cparami \<Rightarrow> assn"
+    and elem_assn :: "'a \<Rightarrow> 'ai \<Rightarrow> assn"
+  assumes lt_impl: "GEN_ALGO pcmp_impl (refines_param_relp cparam_assn elem_assn pcmp)"
+  notes pcmp_aux_hnr[sepref_fr_rules] = gen_refines_param_relpD[OF lt_impl]
+  
+  notes [[sepref_register_adhoc "pcmp"]]
+  
+begin
+
+  thm pcmp_aux_hnr
+  
+  term pcmpo_v_idx2
+  
+  sepref_register pcmpo_idxs2 pcmpo_v_idx2 pcmpo_idx_v2 pcmp_idxs2
+
+  sepref_def pcmpo_idxs_impl [llvm_inline] is "uncurry3 (PR_CONST pcmpo_idxs2)" :: 
+    "cparam_assn\<^sup>k*\<^sub>a(eoarray_assn elem_assn)\<^sup>k *\<^sub>a snat_assn\<^sup>k *\<^sub>a snat_assn\<^sup>k \<rightarrow>\<^sub>a bool1_assn"
+    unfolding pcmpo_idxs2_def PR_CONST_def
+    supply [sepref_fr_rules] = eo_hnr_dep
+    by sepref
+    
+  sepref_def pcmpo_v_idx_impl [llvm_inline] is "uncurry3 (PR_CONST pcmpo_v_idx2)" :: 
+    "cparam_assn\<^sup>k*\<^sub>a(eoarray_assn elem_assn)\<^sup>k *\<^sub>a elem_assn\<^sup>k *\<^sub>a snat_assn\<^sup>k \<rightarrow>\<^sub>a bool1_assn"
+    unfolding pcmpo_v_idx2_def PR_CONST_def
+    supply [sepref_fr_rules] = eo_hnr_dep
+    by sepref
+
+  sepref_def pcmpo_idx_v_impl [llvm_inline] is "uncurry3 (PR_CONST pcmpo_idx_v2)" :: 
+    "cparam_assn\<^sup>k*\<^sub>a(eoarray_assn elem_assn)\<^sup>k *\<^sub>a snat_assn\<^sup>k *\<^sub>a elem_assn\<^sup>k \<rightarrow>\<^sub>a bool1_assn"
+    unfolding pcmpo_idx_v2_def PR_CONST_def
+    supply [sepref_fr_rules] = eo_hnr_dep
+    by sepref
+
+  sepref_def pcmp_idxs_impl [llvm_inline] is "uncurry3 (PR_CONST pcmp_idxs2)" :: 
+    "cparam_assn\<^sup>k*\<^sub>a(woarray_assn elem_assn)\<^sup>k *\<^sub>a snat_assn\<^sup>k *\<^sub>a snat_assn\<^sup>k \<rightarrow>\<^sub>a bool1_assn"
+    unfolding pcmp_idxs2_def PR_CONST_def
+    supply [sepref_fr_rules] = eo_hnr_dep
+    by sepref
+
+
+end  
 
 
 
